add Rows.from_associational and some more length proofs that allow Rows.length_from_associational

src/Experiments/SimplyTypedArithmetic.v
@@ -856,6 +856,8 @@ Module Rows.
                  ) start_state (List.repeat 0 n).
 
     Definition from_columns (inp : cols) : rows := snd (from_columns' (max_column_size inp) (inp, [])).
+
+    Definition from_associational n (p : list (Z * Z)) := from_columns (Columns.from_associational weight n p).
     
     Lemma eval_extract_row (inp : cols): forall n,
         length inp = n ->
@@ -874,10 +876,15 @@ Module Rows.
       destruct x; cbn [hd tl]; rewrite ?sum_nil, ?sum_cons; ring.
     Qed. Hint Rewrite eval_extract_row using (solve [distr_length]) : push_eval.
 
-    Lemma length_extract_row n (inp : cols) :
+    Lemma length_fst_extract_row n (inp : cols) :
       length inp = n -> length (fst (extract_row inp)) = n.
     Proof. cbv [extract_row]; autorewrite with cancel_pair; distr_length. Qed.
-    Hint Rewrite length_extract_row : distr_length.
+    Hint Rewrite length_fst_extract_row : distr_length.
+    
+    Lemma length_snd_extract_row n (inp : cols) :
+      length inp = n -> length (snd (extract_row inp)) = n.
+    Proof. cbv [extract_row]; autorewrite with cancel_pair; distr_length. Qed.
+    Hint Rewrite length_snd_extract_row : distr_length.
 
     (* TODO: move to where list is defined *)
     Hint Rewrite @app_nil_l : list.
@@ -902,20 +909,41 @@ Module Rows.
       rewrite IHinp; distr_length; lia.
     Qed.
 
+    Local Ltac In_cases :=
+      repeat match goal with
+             | H: In _ (_ ++ _) |- _ => apply in_app_or in H; destruct H
+             | H: In _ (_ :: _) |- _ => apply in_inv in H; destruct H
+             | H: In _ nil |- _ => contradiction H
+             end.
+
     Lemma eval_from_columns'_with_length m st n:
       (length (fst st) = n) ->
       length (fst (from_columns' m st)) = n /\
+      ((forall r, In r (snd st) -> length r = n) ->
+       forall r, In r (snd (from_columns' m st)) -> length r = n) /\
       eval n (snd (from_columns' m st)) = Columns.eval weight n (fst st) + eval n (snd st)
                                                                            - Columns.eval weight n (fst (from_columns' m st)).
     Proof.
       cbv [from_columns']; intros.
-      apply fold_right_invariant; intros; [ split; assumption || ring | ].
-      autorewrite with cancel_pair push_eval.
-      split; [ | omega]. apply length_extract_row; tauto.
+      apply fold_right_invariant; intros;
+        repeat match goal with
+               | _ => progress (intros; subst)
+               | _ => progress autorewrite with cancel_pair push_eval
+               | _ => progress In_cases
+               | _ => split; try omega
+               | H: _ /\ _ |- _ => destruct H
+               | _ => solve [auto using length_fst_extract_row, length_snd_extract_row]
+               end.
     Qed.
-    Lemma length_from_columns' m st : length (fst (from_columns' m st)) = length (fst st).
+    Lemma length_fst_from_columns' m st :
+      length (fst (from_columns' m st)) = length (fst st).
     Proof. apply eval_from_columns'_with_length; reflexivity. Qed.
-    Hint Rewrite length_from_columns' : distr_length.
+    Hint Rewrite length_fst_from_columns' : distr_length.
+    Lemma length_snd_from_columns' m st :
+      (forall r, In r (snd st) -> length r = length (fst st)) ->
+      forall r, In r (snd (from_columns' m st)) -> length r = length (fst st).
+    Proof. apply eval_from_columns'_with_length. reflexivity. Qed.
+    Hint Rewrite length_snd_from_columns' : distr_length.
     Lemma eval_from_columns' m st n :
       (length (fst st) = n) -> 
       eval n (snd (from_columns' m st)) = Columns.eval weight n (fst st) + eval n (snd st)
@@ -958,6 +986,32 @@ Module Rows.
                end.
     Qed.
     Hint Rewrite eval_from_columns using (auto; solve [distr_length]) : push_eval.
+
+    Lemma length_from_columns inp:
+      forall r, In r (from_columns inp) -> length r = length inp.
+    Proof.
+      cbv [from_columns]; intros.
+      change inp with (fst (inp, @nil (list Z))).
+      eapply length_snd_from_columns'; eauto.
+      autorewrite with cancel_pair; intros; In_cases.
+    Qed.
+    Hint Rewrite length_from_columns : distr_length.
+
+    Lemma eval_from_associational n p: (n <> 0%nat \/ p = nil) ->
+                                       eval n (from_associational n p) = Associational.eval p.
+    Proof.
+      intros. cbv [from_associational].
+      rewrite eval_from_columns by auto using Columns.length_from_associational.
+      auto using Columns.eval_from_associational.
+    Qed.
+
+    Lemma length_from_associational n p :
+      forall r, In r (from_associational n p) -> length r = n.
+    Proof.
+      cbv [from_associational]; intros.
+      match goal with H: _ |- _ => apply length_from_columns in H end.
+      rewrite Columns.length_from_associational in *; auto.
+    Qed.
 
     Local Notation fw := (fun i => weight (S i) / weight i) (only parsing).
 
@@ -1201,6 +1255,15 @@ Module Rows.
         congruence. }
     Qed.
 
+    Lemma flatten_mod inp n :
+      (forall row, In row inp -> length row = n) ->
+      Positional.eval weight n (fst (flatten inp)) = (eval n inp) mod (weight n).
+    Proof. apply flatten_div_mod. Qed.
+    Lemma flatten_div inp n :
+      (forall row, In row inp -> length row = n) ->
+      snd (flatten inp) = (eval n inp) / (weight n).
+    Proof. apply flatten_div_mod. Qed.
+
     Lemma length_flatten' n start_state inp :
       length (fst start_state) = n ->
       (forall row, In row inp -> length row = n) ->
@@ -1224,7 +1287,7 @@ Module Rows.
                | _ => solve [auto]
                end;
         subst row; distr_length; auto.
-    Qed. Hint Rewrite length_flatten : distr_length. 
+    Qed. Hint Rewrite length_flatten : distr_length.
 
     Lemma flatten'_cons state x inp :
       flatten' state (x :: inp)
